template-coq/theories/utils/MCPartialFuel.v
@@ -1,4 +1,6 @@
 Require Import Coq.Init.Wf.
+Require Import Coq.Wellfounded.Inverse_Image.
+Require Import Coq.Wellfounded.Inclusion.
 Local Set Implicit Arguments.
 Variant PartiallyFueled {R : Prop} {A} := finished (_ : A) | needs_acc (_ : R -> A).
 Arguments PartiallyFueled : clear implicits.
@@ -25,12 +27,38 @@ Definition fully_fuel {R:Prop} {A} (r : R) (v : PartiallyFueled R A) : A
      | finished v => v
      | needs_acc f => f r
      end.
+Definition map_acc {R1 R2 : Prop} (F : R2 -> R1) {A} (v : PartiallyFueled R1 A) : PartiallyFueled R2 A
+  := match v with
+     | finished v => finished v
+     | needs_acc f => needs_acc (fun acc => f (F acc))
+     end.
 
-Definition Fix_fueled {A} {R : A -> A -> Prop} (P : A -> Type)
+Definition Fix_fueled {A} {R : A -> A -> Prop} (P : A -> Type) (Q : forall x : A, P x -> Type)
+           (F : forall (x : A) (p : P x), (forall (y : A) (q : P y), R y x -> PartiallyFueled (well_founded R) (Q y q)) -> PartiallyFueled (well_founded R) (Q x p))
+  : forall (x : A) (p : P x) (fuel : nat), PartiallyFueled (well_founded R) (Q x p)
+  := fix Fix_fueled (x : A) (p : P x) (fuel : nat) : PartiallyFueled (well_founded R) (Q x p)
+    := F x p (fun y q _
+              => match fuel with
+                 | O => needs_acc
+                          (fun rwf
+                           => @Fix A R rwf (fun a => forall (p : P a), Q a p)
+                                   (fun x f p => fully_fuel rwf (F x p (fun y q h => finished (f y h q))))
+                                   y q)
+                 | S fuel' => Fix_fueled y q fuel'
+                 end).
+
+Definition Fix_fueled_simple {A} {R : A -> A -> Prop} (P : A -> Type)
            (F : forall x : A, (forall y : A, R y x -> PartiallyFueled (well_founded R) (P y)) -> PartiallyFueled (well_founded R) (P x))
   : forall (x : A) (fuel : nat), PartiallyFueled (well_founded R) (P x)
-  := fix Fix_fueled (x : A) (fuel : nat) : PartiallyFueled (well_founded R) (P x)
-    := F x (fun y _ => match fuel with
-                       | O => needs_acc (fun rwf => @Fix A R rwf P (fun x f => fully_fuel rwf (F x (fun y h => finished (f y h)))) y)
-                       | S fuel' => Fix_fueled y fuel'
-                       end).
+  := fun x => @Fix_fueled A R (fun _ => unit) (fun x _ => P x) (fun x _ rec => F x ltac:(auto with nocore)) x tt.
+
+Definition on_PartiallyFueled {R A} (P : A -> Prop) (v : PartiallyFueled R A) : Prop
+  := match v with
+     | finished v => P v
+     | needs_acc f => forall acc, P (f acc)
+     end.
+Definition on_partially_fueled {R A} (P : A -> Type) (v : PartiallyFueled R A) : Type
+  := match v with
+     | finished v => P v
+     | needs_acc f => forall acc, P (f acc)
+     end.
